Prove new policy for read replica selection:
previously if one replica became unreachable temporarily, all clients
would stop using it for reads, resulting in an imbalanced
client-to-replica mapping. The only time a client picks a different
preferred replica is when a read on its current replica fails, so any
imbalance created this way would last forever. Now, each client
periodically randomizes its preferred replica to read from so that
balance can be restored on the time scale set by the refresh period.

external/Goose/github_com/mit_pdos/gokv/vrsm/clerk.v
@@ -7,10 +7,14 @@ From Perennial.goose_lang.trusted Require Import github_com.mit_pdos.gokv.truste
 
 From Perennial.goose_lang Require Import ffi.grove_prelude.
 
+(* 1 second *)
+Definition PreferenceRefreshTime : expr := #1000000000.
+
 Definition Clerk := struct.decl [
   "confCk" :: ptrT;
   "replicaClerks" :: slice.T ptrT;
-  "preferredReplica" :: uint64T
+  "preferredReplica" :: uint64T;
+  "lastPreferenceRefresh" :: uint64T
 ].
 
 Definition makeClerks: val :=
@@ -37,6 +41,9 @@ Definition Make: val :=
         struct.storeF Clerk "replicaClerks" "ck" (makeClerks "config");;
         Break));;
     struct.storeF Clerk "preferredReplica" "ck" ((rand.RandomUint64 #()) `rem` (slice.len (struct.loadF Clerk "replicaClerks" "ck")));;
+    let: ("0_ret", "1_ret") := grove_ffi.GetTimeRange #() in
+    struct.storeF Clerk "lastPreferenceRefresh" "ck" "0_ret";;
+    "1_ret";;
     "ck".
 
 (* will retry forever *)
@@ -60,9 +67,22 @@ Definition Clerk__Apply: val :=
         Continue));;
     ![slice.T byteT] "ret".
 
+Definition Clerk__maybeRefreshPreference: val :=
+  rec: "Clerk__maybeRefreshPreference" "ck" :=
+    let: ("now", <>) := grove_ffi.GetTimeRange #() in
+    (if: "now" > ((struct.loadF Clerk "lastPreferenceRefresh" "ck") + PreferenceRefreshTime)
+    then
+      struct.storeF Clerk "preferredReplica" "ck" ((rand.RandomUint64 #()) `rem` (slice.len (struct.loadF Clerk "replicaClerks" "ck")));;
+      let: ("0_ret", "1_ret") := grove_ffi.GetTimeRange #() in
+      struct.storeF Clerk "lastPreferenceRefresh" "ck" "0_ret";;
+      "1_ret";;
+      #()
+    else #()).
+
 Definition Clerk__ApplyRo2: val :=
   rec: "Clerk__ApplyRo2" "ck" "op" :=
     let: "ret" := ref (zero_val (slice.T byteT)) in
+    Clerk__maybeRefreshPreference "ck";;
     Skip;;
     (for: (λ: <>, #true); (λ: <>, Skip) := λ: <>,
       let: "offset" := struct.loadF Clerk "preferredReplica" "ck" in
@@ -80,15 +100,22 @@ Definition Clerk__ApplyRo2: val :=
           Break
         else
           "i" <-[uint64T] ((![uint64T] "i") + #1);;
+          let: ("0_ret", "1_ret") := grove_ffi.GetTimeRange #() in
+          struct.storeF Clerk "lastPreferenceRefresh" "ck" "0_ret";;
+          "1_ret";;
           Continue));;
       (if: (![uint64T] "err") = e.None
       then Break
       else
-        time.Sleep (#10 * #1000000);;
+        let: "timeToSleep" := #5 + ((rand.RandomUint64 #()) `rem` #10) in
+        time.Sleep ("timeToSleep" * #1000000);;
         let: "config" := configservice.Clerk__GetConfig (struct.loadF Clerk "confCk" "ck") in
         (if: (slice.len "config") > #0
         then
           struct.storeF Clerk "replicaClerks" "ck" (makeClerks "config");;
+          let: ("0_ret", "1_ret") := grove_ffi.GetTimeRange #() in
+          struct.storeF Clerk "lastPreferenceRefresh" "ck" "0_ret";;
+          "1_ret";;
           struct.storeF Clerk "preferredReplica" "ck" ((rand.RandomUint64 #()) `rem` (slice.len (struct.loadF Clerk "replicaClerks" "ck")))
         else #());;
         Continue));;
